verified encoding stuff

LeanSAT/Encode/Tseitin.lean
@@ -1,4 +1,4 @@
-import LeanSAT.Encode.EncCNF
+import LeanSAT.Encode.VEncCNF
 
 namespace LeanSAT.Encode.Tseitin
 
@@ -36,12 +36,11 @@ def const (val : Bool) : ReducedForm L b :=
 
 variable {L : Type u} {ν : Type v} [LitVar L ν] in
 mutual
-def reduce : PropForm L → Bool → ReducedForm L b
+def reduce : PropForm ν → Bool → ReducedForm L b
 | .neg f, neg =>
-    have : sizeOf f < 1 + sizeOf f := by simp
     reduce f (!neg)
 | .var l, neg =>
-    .lit (if neg then (-l) else l)
+    .lit <| LitVar.mkLit _ l (!neg)
 | .tr, neg =>
     const (!neg)
 | .fls, neg =>
@@ -55,17 +54,17 @@ def reduce : PropForm L → Bool → ReducedForm L b
     then reduceConj x y true
     else reduceDisj x y false
 | .impl h c, neg =>
-    reduce (.disj (.neg h) c) neg
+    reduce (.disj c (.neg h)) neg
 | .biImpl l r, neg =>
     reduce (.conj (.impl l r) (.impl r l)) neg
 
-def reduceConj [LitVar L ν] (x y : PropForm L) (neg : Bool) : ReducedForm L b :=
+def reduceConj (x y : PropForm ν) (neg : Bool) : ReducedForm L b :=
   let blah := .and <| (reduce x neg).conjuncts ++ (reduce y neg).conjuncts
   match b with
   | true  => blah
   | false => .or #[blah]
 
-def reduceDisj [LitVar L ν] (x y : PropForm L) (neg : Bool) : ReducedForm L b :=
+def reduceDisj (x y : PropForm ν) (neg : Bool) : ReducedForm L b :=
   let blah := .or <| (reduce x neg).disjuncts ++ (reduce y neg).disjuncts
   match b with
   | true  => .and #[blah]
@@ -76,26 +75,136 @@ termination_by
   reduceConj x y neg => reduceSize x + reduceSize y
   reduceDisj x y neg => reduceSize x + reduceSize y
 
-def tseitin (f : PropForm ILit) : EncCNF Unit := do
-  let red := reduce f true
-  topAnd red
+def ReducedForm.toPropFun [LitVar L V] (r : ReducedForm L b) : PropFun V :=
+  match r with
+  | and fs =>
+    let fs' := fs.attach.map (fun ⟨x,_h⟩ => ReducedForm.toPropFun x)
+    PropFun.all fs'
+  | or fs  =>
+    let fs' := fs.attach.map (fun ⟨x,_h⟩ => ReducedForm.toPropFun x)
+    PropFun.any fs'
+  | lit l => LitVar.toPropFun l
+
+@[simp] theorem const_toPropFun [LitVar L ν]
+  : (const b1 : ReducedForm L b2).toPropFun = if b1 then ⊤ else ⊥
+  := by
+  ext τ
+  cases b1 <;> cases b2 <;> (
+    simp [const]
+    simp [ReducedForm.toPropFun, Array.mem_def, Array.attach]
+  )
+
+theorem ReducedForm.conjuncts_toPropFun [LitVar L ν] (r : ReducedForm L true)
+  : r.toPropFun = (PropFun.all (r.conjuncts.map toPropFun)) :=
+  match r with
+  | .and rs => by ext τ; simp [conjuncts, Array.mem_def, Array.attach, toPropFun]
+  | .lit l => by ext τ; simp [conjuncts, Array.mem_def]; rfl
+
+theorem ReducedForm.disjuncts_toPropFun [LitVar L ν] (r : ReducedForm L false)
+  : r.toPropFun = (PropFun.any (r.disjuncts.map toPropFun)) :=
+  match r with
+  | .or rs => by ext τ; simp [disjuncts, Array.mem_def, Array.attach, toPropFun]
+  | .lit l => by ext τ; simp [disjuncts, Array.mem_def]; rfl
+
+/- TODO: This proof is really slow... -/
+set_option maxHeartbeats 500000 in
+open PropFun in
+variable {L : Type u} {ν : Type v} [LitVar L ν] [LawfulLitVar L ν] in
+mutual
+def reduce_toPropFun (f : PropForm ν) (neg : Bool)
+  : (reduce f neg : ReducedForm L b).toPropFun = ⟦ if neg then .neg f else f ⟧ :=
+  match f with
+  | .neg f =>
+      have := reduce_toPropFun f (!neg)
+      by simp [reduce]; rw [this]; cases neg <;> simp
+  | .var l => by
+      simp [reduce]
+      cases neg <;> simp [ReducedForm.toPropFun, LitVar.toPropFun]
+  | .tr => by
+      simp [reduce]
+      cases neg <;> simp
+  | .fls => by
+      simp [reduce]
+      cases neg <;> simp
+  | .conj x y =>
+      have h1 := reduceDisj_toPropFun x y true
+      have h2 := reduceConj_toPropFun x y false
+      by simp [reduce]; cases neg <;> simp <;> (first | rw [h1] | rw [h2]) <;> simp
+  | .disj x y =>
+      have h1 := reduceConj_toPropFun x y true
+      have h2 := reduceDisj_toPropFun x y false
+      by simp [reduce]; cases neg <;> simp <;> (first | rw [h1] | rw [h2]) <;> simp
+  | .impl h c =>
+      have h' := reduce_toPropFun (b := b) (.disj c (.neg h)) neg
+      by unfold reduce; rw [h']; clear h'
+         cases neg <;> simp [BooleanAlgebra.sdiff_eq, BooleanAlgebra.himp_eq]
+  | .biImpl l r =>
+      have h' := reduce_toPropFun (b := b) (.conj (.impl l r) (.impl r l)) neg
+      by unfold reduce; rw [h']; clear h'
+         cases neg <;> simp [biImpl_eq_impls, BooleanAlgebra.sdiff_eq, BooleanAlgebra.himp_eq]
+
+def reduceConj_toPropFun (x y : PropForm ν) (neg : Bool)
+  : (reduceConj x y neg : ReducedForm L b).toPropFun =
+      ⟦ if neg then .neg (.disj x y) else (.conj x y) ⟧
+  := by
+  have h1 := reduce_toPropFun (b := true) x neg
+  have h2 := reduce_toPropFun (b := true) y neg
+  ext τ
+  have := congrArg (τ ⊨ ·) <| ReducedForm.conjuncts_toPropFun (L := L) (reduce x neg)
+  rw [h1] at this
+  have := congrArg (τ ⊨ ·) <| ReducedForm.conjuncts_toPropFun (L := L) (reduce y neg)
+  rw [h2] at this
+  clear h1 h2
+  cases b <;> (
+    simp [reduceConj]
+    simp [ReducedForm.toPropFun, Array.mem_def, Array.attach] at *
+    aesop
+  )
+
+
+def reduceDisj_toPropFun (x y : PropForm ν) (neg : Bool)
+  : (reduceDisj x y neg : ReducedForm L b).toPropFun =
+    ⟦ if neg then .neg (.conj x y) else .disj x y ⟧
+  := by
+  have h1 := reduce_toPropFun (b := false) x neg
+  have h2 := reduce_toPropFun (b := false) y neg
+  ext τ
+  have := congrArg (τ ⊨ ·) <| ReducedForm.disjuncts_toPropFun (L := L) (reduce x neg)
+  rw [h1] at this
+  have := congrArg (τ ⊨ ·) <| ReducedForm.disjuncts_toPropFun (L := L) (reduce y neg)
+  rw [h2] at this
+  clear h1 h2
+  cases b <;> (
+    simp [reduceDisj]
+    simp [ReducedForm.toPropFun, Array.mem_def, Array.attach] at *
+    cases neg <;> (
+      simp_all; clear this; clear this
+      generalize ReducedForm.disjuncts _ = xr
+      generalize ReducedForm.disjuncts _ = yr
+      cases xr; cases yr
+      aesop
+    )
+  )
+end
+termination_by
+  reduce_toPropFun f neg => reduceSize f
+  reduceConj_toPropFun x y neg => reduceSize x + reduceSize y
+  reduceDisj_toPropFun x y neg => reduceSize x + reduceSize y
+
+
+
+def tseitin [LitVar L V] [LawfulLitVar L V] [DecidableEq V] [Fintype V]
+      (f : PropForm V) : VEncCNF L ⟦f⟧ Unit :=
+  let red : ReducedForm L true := reduce f false
+  VEncCNF.withTemps 1 (
+    aux red
+  ) |>.mapProp (by
+    simp; rw [reduce_toPropFun]; simp
+  )
 where
-  topAnd : ReducedForm ILit true → EncCNF Unit
-    | .and fs => do
-      let cs : Array IClause ← fs.subtypeSize.mapM (fun ⟨f,h⟩ =>
-        have := Nat.le_trans h (Nat.le_add_left _ 1)
-        topOr f)
-      for c in cs do
-        addClause c
-    | .lit l => addClause #[l]
-  topOr : ReducedForm ILit false → EncCNF IClause
-    | .or fs => do
-      let cs : Array ILit ← fs.subtypeSize.mapM (fun ⟨f,h⟩ =>
-        have := Nat.le_trans h (Nat.le_add_left _ 1)
-        aux f)
-      return cs
-    | .lit l => return #[l]
-  aux {b} : ReducedForm ILit b → EncCNF ILit
+  aux {b} (f : ReducedForm L b) : VEncCNF (WithTemps L 1)
+        (.biImpl (.var (Sum.inr 0)) (f.toPropFun.map Sum.inl)) Unit :=
+    match f with
     | .lit l => pure l
     | .and fs => do
       let ls : Array ILit ← fs.subtypeSize.mapM (fun ⟨f,h⟩ =>
