LeanSAT/Encode/VEncCNF.lean
@@ -1,0 +1,172 @@
+/- Copyright (c) the LeanSAT contributors.
+
+Authors: James Gallicchio
+-/
+
+import LeanSAT.Encode.EncCNF
+
+/-! # Verified Encodings
+
+This file defines `VEncCNF`,
+the main type for building *verified* encodings to CNF.
+This augments the regular `EncCNF` with the ability to specify
+and verify what a particular `EncCNF` value actually encodes.
+-/
+
+namespace LeanSAT.Encode
+
+open Model PropFun EncCNF
+
+def EncCNF.satisfiesProp [LitVar L ν] (e : EncCNF L α) (P : PropFun ν) : Prop :=
+  ∀ s,
+    let (a,s') := (e.1 s)
+    s'.vMap = s.vMap ∧
+    s'.assumeVars = s.assumeVars ∧
+    s'.interp = (s.interp ⊓ ((s.assumeVars.toPropFun)ᶜ ⇨ P))
+
+def VEncCNF (L : Type u) [LitVar L ν] (α : Type u) (P : PropFun ν) :=
+  { e : EncCNF L α // e.satisfiesProp P }
+
+namespace VEncCNF
+
+variable {L} [LitVar L ν]
+
+instance : CoeHead (VEncCNF L α P) (EncCNF L α) := ⟨(·.1)⟩
+
+def mapProp {P P' : PropFun ν} (h : P = P') : VEncCNF L α P → VEncCNF L α P' :=
+  fun ⟨e,he⟩ => ⟨e, h ▸ he⟩
+
+def newCtx (name : String) (inner : VEncCNF L α P) : VEncCNF L α P :=
+  ⟨EncCNF.newCtx name inner, inner.2⟩
+
+def addClause [DecidableEq ν] (C : Clause L) : VEncCNF L Unit (C.toPropFun) :=
+  ⟨EncCNF.addClause C, by
+    intro s
+    generalize he : (EncCNF.addClause C).1 s = e
+    rcases e with ⟨_,s'⟩
+    simp
+    simp [EncCNF.addClause] at he; cases he; simp
+    ext τ
+    simp [EncCNF.LawfulState.interp]
+    simp [PropFun.satisfies_invImage]
+    have : ∀ {_ _ _}, _ := @PropFun.invImage_setManyMap_map_idem (f := s.1.vMap) (h := s.vMapInj) (τ := τ)
+    constructor
+    · rintro ⟨τ',h1,h2⟩
+      refine ⟨⟨τ',h1⟩,?_⟩
+      rw [this] at h2
+      rcases h2 with (h2|h2)
+        <;> simp [h2]
+    · rintro ⟨⟨τ',h1⟩,h2⟩
+      refine ⟨τ',?_⟩
+      simp [*]
+      by_cases τ ⊨ s.assumeVars.toPropFun
+      · simp [*]
+      · simp [*]
+    ⟩
+
+/-- runs `e`, adding `ls` to each generated clause -/
+def unlessOneOf [LawfulLitVar L ν] (ls : Array L) (ve : VEncCNF L α P)
+    : VEncCNF L α ((Cnf.not ls).toPropFun ⇨ P) :=
+  ⟨EncCNF.unlessOneOf ls ve, by
+    -- TODO: terrible, slow proof
+    intro s
+    rcases ve with ⟨ve,hve⟩
+    simp [StateT.run] at hve ⊢
+    generalize he : (EncCNF.unlessOneOf ls ve).1 s = e
+    rcases e with ⟨a,s'⟩; dsimp
+    simp [EncCNF.unlessOneOf] at he
+    generalize hsprev : EncCNF.LawfulState.mk .. = sprev at he
+    generalize he' : ve.1 sprev = e
+    rcases e with ⟨a',s''⟩
+    have := hve sprev; clear hve
+    simp [he'] at he this
+    clear he'
+    cases he; cases hsprev
+    rcases s'' with ⟨⟨s''a,s''b,s''c⟩,s''d,s''e,s''f⟩
+    rcases s with ⟨⟨sa,sb,sc⟩,sd,se,sf⟩
+    simp_all
+    cases this
+    subst_vars
+    simp [EncCNF.LawfulState.interp] at *
+    simp_all
+    clear! s''f s''e s''d sf se sd
+    ext τ
+    simp
+    apply Function.const
+    clear! sa sb sc s''a s''b
+    push_neg
+    exact and_imp⟩
+
+def assuming [LawfulLitVar L ν] (ls : Array L) (e : VEncCNF L α P)
+    : VEncCNF L α ((Cnf.all ls).toPropFun ⇨ P) :=
+  unlessOneOf (ls.map (- ·)) e |>.mapProp (by
+    ext τ
+    simp [Clause.satisfies_iff, Array.mem_def]
+  )
+
+noncomputable def withTemps.prop [DecidableEq ν] [Fintype ν] (P : PropFun (ν ⊕ Fin n)) :=
+  P.invImage ⟨Sum.inl,Sum.inl_injective⟩ Finset.univ
+
+--theorem withTemps.prop_of_
+
+set_option pp.proofs.withType false in
+def withTemps [DecidableEq ν] [Fintype ν] (n) {P : PropFun (ν ⊕ Fin n)}
+    (e : VEncCNF (WithTemps L n) α P) :
+    VEncCNF L α (withTemps.prop P) :=
+  ⟨EncCNF.withTemps _ e.1, by
+    intro s
+    rcases e with ⟨e,he⟩
+    generalize hs' : (EncCNF.withTemps n e).1 s = res
+    rcases res with ⟨a,s'⟩
+    simp [EncCNF.withTemps] at hs'
+    simp
+    split at hs'; next a s'' hs'' =>
+    cases hs'
+    have := he (LawfulState.withTemps s); clear he; have he := this; clear this
+    rw [hs''] at he
+    simp at he ⊢
+    rcases s'' with ⟨⟨nv,cnf,vm,av⟩,cvlt,vmlt,vmi⟩
+    simp [LawfulState.withTemps, State.withTemps, LawfulState.interp] at he
+    rcases he with ⟨rfl,rfl,he⟩
+    simp [LawfulState.withoutTemps, State.withoutTemps, LawfulState.interp]
+    ext τ
+    have : ∀ τ' : PropAssignment _, τ' ⊨ _ ↔ τ' ⊨ _ ⊓ _ :=
+        fun _ => iff_of_eq <| congrArg _ he
+    clear he
+    simp [PropFun.satisfies_invImage] at this ⊢
+    constructor
+    · rintro ⟨τ',h⟩
+      have := this τ'
+    · rintro ⟨τ',h⟩
+      sorry⟩
+
+theorem bind_satisfiesProp (e1 : EncCNF L α) (e2 : α → EncCNF L β)
+  : e1.satisfiesProp P → (∀ s, (e2 (e1.1 s).1).satisfiesProp Q) →
+    (do let a ← e1.1; (e2 a).1).satisfiesProp (P ⊓ Q)
+  := by
+  intro s
+  rcases ve1 with ⟨⟨s1,_⟩,he1⟩
+  have := he1 s
+  simp [Bind.bind, StateT.bind] at this ⊢
+  clear he1; have he1 := this; clear this
+  generalize hs' : s1 s = res' at he1 ⊢
+  rcases res' with ⟨a,s'⟩
+  simp at he1 ⊢
+  generalize ve2 a = ve2
+  rcases ve2 with ⟨⟨s2,_⟩,he2⟩
+  have := he2 s'
+  simp at this ⊢
+  clear he2; have he2 := this; clear this
+  generalize hs'' : s2 s' = res' at he2 ⊢
+  rcases res' with ⟨b,s''⟩
+  simp at he2 ⊢
+  simp [*]
+  rw [inf_assoc]; congr
+  exact (himp_inf_distrib ..).symm
+
+def seq (e1 : VEncCNF L α P) (e2 : VEncCNF L β Q) : VEncCNF L (α × β) (P ⊓ Q) :=
+  ⟨ do let a ← e1; let b ← e2; return (a,b)
+  , by
+    apply bind_satisfiesProp
+    sorry
+    ⟩
